sim almost done, refactor

imp/Imp2Csharpminor.v
@@ -15,9 +15,6 @@ From compcert Require Import
 
 From compcert Require Compiler.
 
-(* From compcert Require Import Cminor Cminortyping. *)
-(* Import RTLtypes. *)
-
 Import Int.
 
 Set Implicit Arguments.
@@ -333,28 +330,11 @@ Section Compile.
     end
   .
 
-  Definition _compile2 (src : Imp.programL) : res program :=
-    let optdefs := (compile_gdefs src) in
-    match optdefs with
-    | None => Error [MSG "Imp2csharpminor compilation failed"]
-    | Some _defs =>
-      if (Coqlib.list_norepet_dec dec (List.map fst _defs)) then
-        OK (mkprogram _defs (List.map s2p src.(publicL)) (s2p "main"))
-      else Error [MSG "Imp2csharpminor compilation failed; duplicated declarations"]
-    end
-  .
-
 End Compile.
 
 Definition compile (src : Imp.programL) :=
   match (get_gmap src) with
   | Some gm => _compile gm src
-  | _ => Error [MSG "Imp2csharpminor compilation failed"]
-  end.
-
-Definition compile2 (src : Imp.programL) :=
-  match (get_gmap src) with
-  | Some gm => _compile2 gm src
   | _ => Error [MSG "Imp2csharpminor compilation failed"]
   end.
 
@@ -377,125 +357,11 @@ Module ASMGEN.
 
 End ASMGEN.
 
-Definition extFun_Dec : forall x y : (string * nat), {x = y} + {x <> y}.
-Proof.
-  i. destruct x, y.
-  assert (NC: {n = n0} + {n <> n0}); auto using nat_Dec.
-  assert (SC: {s = s0} + {s <> s0}); auto using string_Dec.
-  destruct NC; destruct SC; clarify; auto.
-  all: right; intros p; apply pair_equal_spec in p; destruct p; clarify.
-Qed.
-
-Section Link.
-
-  Variable src1 : Imp.programL.
-  Variable src2 : Imp.programL.
-
-  Let l_nameL := src1.(nameL) ++ src2.(nameL).
-  Let l_prog_varsL := src1.(prog_varsL) ++ src2.(prog_varsL).
-  Let l_prog_funsLM := src1.(prog_funsL) ++ src2.(prog_funsL).
-  Let l_prog_funsL := List.map snd l_prog_funsLM.
-  Let l_publicL := src1.(publicL) ++ src2.(publicL).
-  Let l_defsL := src1.(defsL) ++ src2.(defsL).
-
-  Let check_name_unique1 {K} {A} {B} decK
-      (l1 : list (K * A)) (l2 : list (K * B)) :=
-    let l1_k := List.map fst l1 in
-    let l2_k := List.map fst l2 in
-    Coqlib.list_norepet_dec decK (l1_k ++ l2_k).
-
-  (* check defined names are unique *)
-  Definition link_imp_cond1 :=
-    check_name_unique1 string_Dec l_prog_varsL l_prog_funsL.
-
-  Let check_name_unique2 {K} {B} decK
-      (l1 : list K) (l2 : list (K * B)) :=
-    let l2_k := List.map fst l2 in
-    Coqlib.list_norepet_dec decK (l1 ++ l2_k).
-
-  (* check external decls are consistent *)
-  Definition link_imp_cond2 :=
-    let sd := string_Dec in
-    let c1 := check_name_unique2 sd src1.(ext_varsL) l_prog_funsL in
-    let c2 := check_name_unique2 sd src2.(ext_varsL) l_prog_funsL in
-    let c3 := check_name_unique1 sd src1.(ext_funsL) l_prog_varsL in
-    let c4 := check_name_unique1 sd src2.(ext_funsL) l_prog_varsL in
-    c1 && c2 && c3 && c4.
-
-  (* check external fun decls' sig *)
-  Fixpoint _link_imp_cond3' (p : string * nat) (l : extFuns) :=
-    let '(name, n) := p in
-    match l with
-    | [] => true
-    | (name2, n2) :: t =>
-      if (eqb name name2 && negb (n =? n2)) then false
-      else _link_imp_cond3' p t
-    end
-  .
-
-  Fixpoint _link_imp_cond3 l :=
-    match l with
-    | [] => true
-    | h :: t =>
-      if (_link_imp_cond3' h t) then _link_imp_cond3 t
-      else false
-    end
-  .
-
-  Definition link_imp_cond3 :=
-    _link_imp_cond3 (src1.(ext_funsL) ++ src2.(ext_funsL)).
-
-  (* merge external decls; vars is simple, funs assumes cond3 is passed *)
-  Let l_ext_vars0 := nodup string_Dec (src1.(ext_varsL) ++ src2.(ext_varsL)).
-
-  Let l_ext_funs0 := nodup extFun_Dec (src1.(ext_funsL) ++ src2.(ext_funsL)).
-
-  (* link external decls; need to remove defined names *)
-  Let l_ext_vars :=
-    let l_prog_varsL' := List.map fst l_prog_varsL in
-    filter (fun s => negb (in_dec string_Dec s l_prog_varsL')) l_ext_vars0.
-
-  Let l_ext_funs :=
-    let l_prog_funsL' := List.map fst l_prog_funsL in
-    filter (fun sn => negb (in_dec string_Dec (fst sn) l_prog_funsL')) l_ext_funs0.
-
-  (* Linker for Imp programs, follows Clight's link_prog as possible *)
-  Definition link_imp : option Imp.programL :=
-    if (link_imp_cond1 && link_imp_cond2 && link_imp_cond3)
-    then Some (mk_programL l_nameL l_ext_vars l_ext_funs l_prog_varsL l_prog_funsLM l_publicL l_defsL)
-    else None
-  .
-
-End Link.
-
 Section Beh.
-
-  (* Definition map_val (v : eventval) : option val := *)
-  (*   match v with *)
-  (*   | EVlong vl => Some (Vint vl.(Int64.intval)) *)
-  (*   | _ => None *)
-  (*   end. *)
 
   Inductive match_val : eventval -> val -> Prop :=
   | match_val_intro :
       forall v, match_val (EVlong v) (Vint (Int64.signed v)).
-
-  (* Fixpoint map_vals (vlist : list eventval) acc : option (list val) := *)
-  (*   match vlist with *)
-  (*   | [] => Some acc *)
-  (*   | v :: t => do mv <- map_val v; map_vals t (acc ++ [mv]) *)
-  (*   end. *)
-
-  (* Definition match_vals : list eventval -> list val -> Prop := List.Forall2 match_val. *)
-
-  (* Definition map_event (ev : Events.event) : option Universe.event := *)
-  (*   match ev with *)
-  (*   | Event_syscall name args r => *)
-  (*     do margs <- map_vals args []; *)
-  (*     do mr <- map_val r; *)
-  (*     Some (event_sys name margs mr) *)
-  (*   | _ => None *)
-  (*   end. *)
 
   Inductive match_event : Events.event -> Universe.event -> Prop :=
   | match_event_intro
@@ -505,34 +371,6 @@ Section Beh.
     :
       match_event (Event_syscall name eargs er) (event_sys name uargs ur)
   .
-
-  (* Fixpoint map_trace (tr : trace) acc : option (list Universe.event) := *)
-  (*   match tr with *)
-  (*   | [] => Some acc *)
-  (*   | ev :: t => *)
-  (*     do mev <- map_event ev; map_trace t (acc ++ [mev]) *)
-  (*   end. *)
-
-  (* Definition match_trace : trace -> list Universe.event -> Prop := List.Forall2 match_event. *)
-
-  (* Inductive match_beh : program_behavior -> Tr.t -> Prop := *)
-  (* | match_beh_Terminates : *)
-  (*     forall tr mtr r, *)
-  (*       map_trace tr [] = Some mtr -> *)
-  (*       match_beh (Terminates tr r) (Tr.app mtr (Tr.done r.(intval))) *)
-  (* | match_beh_Diverges : *)
-  (*     forall tr mtr, *)
-  (*       map_trace tr [] = Some mtr -> *)
-  (*       match_beh (Diverges tr) (Tr.app mtr (Tr.spin)) *)
-  (* | match_beh_Reacts : *)
-  (*     forall ev mev trinf mt, *)
-  (*       map_event ev = Some mev -> *)
-  (*       match_beh (Reacts trinf) mt -> *)
-  (*       match_beh (Reacts (Econsinf ev trinf)) (Tr.cons mev mt) *)
-  (* | match_beh_Goes_wrong : *)
-  (*     forall tr mtr, *)
-  (*       map_trace tr [] = Some mtr -> *)
-  (*       match_beh (Goes_wrong tr) (Tr.app mtr (Tr.ub)). *)
 
   Variant _match_beh (match_beh: _ -> _ -> Prop) (tgtb : program_behavior) (srcb : Tr.t) : Prop :=
   | match_beh_Terminates
