imp/Imp2CsharpminorLink.v
@@ -1,0 +1,103 @@
+Require Import Coqlib.
+Require Import Universe.
+Require Import Skeleton.
+Require Import PCM.
+Require Import STS Behavior.
+Require Import Any.
+Require Import ModSem.
+Require Import Imp.
+
+From compcert Require Import AST Csharpminor Globalenvs Linking.
+
+Set Implicit Arguments.
+
+Definition extFun_Dec : forall x y : (string * nat), {x = y} + {x <> y}.
+Proof.
+  i. destruct x, y.
+  assert (NC: {n = n0} + {n <> n0}); auto using nat_Dec.
+  assert (SC: {s = s0} + {s <> s0}); auto using string_Dec.
+  destruct NC; destruct SC; clarify; auto.
+  all: right; intros p; apply pair_equal_spec in p; destruct p; clarify.
+Qed.
+
+Section Link.
+
+  Variable src1 : Imp.programL.
+  Variable src2 : Imp.programL.
+
+  Let l_nameL := src1.(nameL) ++ src2.(nameL).
+  Let l_prog_varsL := src1.(prog_varsL) ++ src2.(prog_varsL).
+  Let l_prog_funsLM := src1.(prog_funsL) ++ src2.(prog_funsL).
+  Let l_prog_funsL := List.map snd l_prog_funsLM.
+  Let l_publicL := src1.(publicL) ++ src2.(publicL).
+  Let l_defsL := src1.(defsL) ++ src2.(defsL).
+
+  Let check_name_unique1 {K} {A} {B} decK
+      (l1 : list (K * A)) (l2 : list (K * B)) :=
+    let l1_k := List.map fst l1 in
+    let l2_k := List.map fst l2 in
+    Coqlib.list_norepet_dec decK (l1_k ++ l2_k).
+
+  (* check defined names are unique *)
+  Definition link_imp_cond1 :=
+    check_name_unique1 string_Dec l_prog_varsL l_prog_funsL.
+
+  Let check_name_unique2 {K} {B} decK
+      (l1 : list K) (l2 : list (K * B)) :=
+    let l2_k := List.map fst l2 in
+    Coqlib.list_norepet_dec decK (l1 ++ l2_k).
+
+  (* check external decls are consistent *)
+  Definition link_imp_cond2 :=
+    let sd := string_Dec in
+    let c1 := check_name_unique2 sd src1.(ext_varsL) l_prog_funsL in
+    let c2 := check_name_unique2 sd src2.(ext_varsL) l_prog_funsL in
+    let c3 := check_name_unique1 sd src1.(ext_funsL) l_prog_varsL in
+    let c4 := check_name_unique1 sd src2.(ext_funsL) l_prog_varsL in
+    c1 && c2 && c3 && c4.
+
+  (* check external fun decls' sig *)
+  Fixpoint _link_imp_cond3' (p : string * nat) (l : extFuns) :=
+    let '(name, n) := p in
+    match l with
+    | [] => true
+    | (name2, n2) :: t =>
+      if (eqb name name2 && negb (n =? n2)%nat) then false
+      else _link_imp_cond3' p t
+    end
+  .
+
+  Fixpoint _link_imp_cond3 l :=
+    match l with
+    | [] => true
+    | h :: t =>
+      if (_link_imp_cond3' h t) then _link_imp_cond3 t
+      else false
+    end
+  .
+
+  Definition link_imp_cond3 :=
+    _link_imp_cond3 (src1.(ext_funsL) ++ src2.(ext_funsL)).
+
+  (* merge external decls; vars is simple, funs assumes cond3 is passed *)
+  Let l_ext_vars0 := nodup string_Dec (src1.(ext_varsL) ++ src2.(ext_varsL)).
+
+  Let l_ext_funs0 := nodup extFun_Dec (src1.(ext_funsL) ++ src2.(ext_funsL)).
+
+  (* link external decls; need to remove defined names *)
+  Let l_ext_vars :=
+    let l_prog_varsL' := List.map fst l_prog_varsL in
+    List.filter (fun s => negb (in_dec string_Dec s l_prog_varsL')) l_ext_vars0.
+
+  Let l_ext_funs :=
+    let l_prog_funsL' := List.map fst l_prog_funsL in
+    List.filter (fun sn => negb (in_dec string_Dec (fst sn) l_prog_funsL')) l_ext_funs0.
+
+  (* Linker for Imp programs, follows Clight's link_prog as possible *)
+  Definition link_imp : option Imp.programL :=
+    if (link_imp_cond1 && link_imp_cond2 && link_imp_cond3)
+    then Some (mk_programL l_nameL l_ext_vars l_ext_funs l_prog_varsL l_prog_funsLM l_publicL l_defsL)
+    else None
+  .
+
+End Link.
