imp/Imp2CsharpminorSepComp.v
@@ -1,0 +1,192 @@
+From compcert Require Import Globalenvs Smallstep AST Integers Events Behaviors Errors Memory Csharpminor Linking.
+Require Import Coqlib.
+Require Import ITreelib.
+Require Import Universe.
+Require Import Skeleton.
+Require Import PCM.
+Require Import STS Behavior.
+Require Import Any.
+Require Import ModSem.
+Require Import Imp.
+Require Import Imp2Csharpminor.
+Require Import ImpProofs.
+Require Import SimSTS2.
+Require Import Mem0.
+Require Import IRed.
+
+Require Import Imp2CsharpminorMatch.
+Require Import Imp2CsharpminorArith.
+Require Import Imp2CsharpminorGenv.
+Require Import Imp2CsharpminorMem.
+Require Import Imp2CsharpminorLink.
+Require Import Imp2CsharpminorSim.
+
+Set Implicit Arguments.
+
+Section PROOFALL.
+
+  Import Maps.PTree.
+
+  (* Lemma list_norepet_NoDupB {K} {decK} : *)
+  (*   forall l, Coqlib.list_norepet l <-> @NoDupB K decK l = true. *)
+  (* Proof. *)
+  (*   split; i. *)
+  (*   - induction H; ss. *)
+  (*     clarify. *)
+  (*     destruct (in_dec decK hd tl); clarify. *)
+  (*   - induction l; ss; clarify. constructor. *)
+  (*     des_ifs. econs 2; auto. *)
+  (* Qed. *)
+
+  (* Definition wf_imp_prog (src : Imp.programL) := *)
+  (*   Coqlib.list_norepet (compile_gdefs (get_gmap src) src). *)
+
+  (* Lemma compile_then_wf : forall src tgt, *)
+  (*     compile src = OK tgt *)
+  (*     -> *)
+  (*     wf_imp_prog src. *)
+  (* Proof. *)
+  (*   unfold compile, _compile. i. *)
+  (*   destruct (compile_gdefs (get_gmap src) src) eqn:EQ; clarify. *)
+  (*   eauto using compile_gdefs_then_wf. *)
+  (* Qed. *)
+
+  (* Maps.PTree.elements_extensional 
+     we will rely on above theorem for commutation lemmas *)
+  Lemma _comm_link_imp_compile
+        src1 src2 srcl tgt1 tgt2 tgtl
+        (COMP1: compile src1 = OK tgt1)
+        (COMP2: compile src2 = OK tgt2)
+        (LINKSRC: link_imp src1 src2 = Some srcl)
+        (LINKTGT: link_prog tgt1 tgt2 = Some tgtl)
+    :
+      <<COMPL: compile srcl = OK tgtl>>.
+  Proof.
+  Admitted.
+
+  Definition wf_link {T} (program_list : list T) :=
+    exists h t, program_list = h :: t.
+
+  Inductive compile_list :
+    list programL -> list (Csharpminor.program) -> Prop :=
+  | compile_nil :
+      compile_list [] []
+  | compile_head
+      src_h src_t tgt_h tgt_t
+      (COMPH: compile src_h = OK tgt_h)
+      (COMPT: compile_list src_t tgt_t)
+    :
+      <<COMPLIST: compile_list (src_h :: src_t) (tgt_h :: tgt_t)>>.
+
+  Definition fold_left_option {T} f (t : list T) (opth : option T) :=
+    fold_left
+      (fun opt s2 => match opt with | Some s1 => f s1 s2 | None => None end)
+      t opth.
+
+  Lemma fold_left_option_None {T} :
+    forall f (l : list T), fold_left_option f l None = None.
+  Proof.
+    intros f. induction l; ss; clarify.
+  Qed.
+
+  Definition link_imp_list src_list :=
+    match src_list with
+    | [] => None
+    | src_h :: src_t =>
+      fold_left_option link_imp src_t (Some src_h)
+    end.
+
+  Definition link_csm_list (tgt_list : list (Csharpminor.program)) :=
+    match tgt_list with
+    | [] => None
+    | tgt_h :: tgt_t =>
+      fold_left_option link_prog tgt_t (Some tgt_h)
+    end.
+
+  Lemma comm_link_imp_compile
+        src_list srcl tgt_list tgtl
+        (COMPL: compile_list src_list tgt_list)
+        (LINKSRC: link_imp_list src_list = Some srcl)
+        (LINKTGT: link_csm_list tgt_list = Some tgtl)
+    :
+      compile srcl = OK tgtl.
+  Proof.
+    i. destruct src_list; destruct tgt_list; ss; clarify.
+    inv COMPL; clarify.
+    generalize dependent srcl. generalize dependent tgtl.
+    generalize dependent p. generalize dependent p0.
+    induction COMPT; i; ss; clarify.
+    destruct (link_prog p0 tgt_h) eqn:LPt; ss; clarify.
+    2:{ rewrite fold_left_option_None in LINKTGT; clarify. }
+    destruct (link_imp p src_h) eqn:LPs; ss; clarify.
+    2:{ rewrite fold_left_option_None in LINKSRC; clarify. }
+    eapply IHCOMPT.
+    2: apply LINKTGT.
+    2: apply LINKSRC.
+    eapply _comm_link_imp_compile.
+    3: apply LPs.
+    3: apply LPt.
+    auto. auto.
+  Qed.
+
+  Context `{Σ: GRA.t}.
+
+  Lemma _comm_link_imp_link_mod
+        src1 src2 srcl tgt1 tgt2 tgtl (ctx : ModL.t)
+        (MOD1: ImpMod.get_modL src1 = tgt1)
+        (MOD2: ImpMod.get_modL src2 = tgt2)
+        (LINKIMP: link_imp src1 src2 = Some srcl)
+        (MODL: ImpMod.get_modL srcl = tgtl)
+    :
+      <<LINKMOD: ModL.add (ModL.add ctx tgt1) tgt2 = ModL.add ctx tgtl>>.
+  Proof.
+  Admitted.
+
+  Lemma comm_link_imp_link_mod
+        src_list srcl tgt_list tgtl ctx
+        (MODLIST: List.map (fun src => ImpMod.get_modL src) src_list = tgt_list)
+        (LINKIMP: link_imp_list src_list = Some srcl)
+        (MODL: ImpMod.get_modL srcl = tgtl)
+    :
+      <<LINKMOD: fold_left ModL.add tgt_list ctx = ModL.add ctx tgtl>>.
+  Proof.
+    destruct src_list eqn:SL; i; ss; clarify.
+    move p after l.
+    revert_until Σ.
+    induction l; i; ss; clarify.
+    destruct (link_imp p a) eqn:LI; ss; clarify.
+    2:{ rewrite fold_left_option_None in LINKIMP; clarify. }
+    erewrite _comm_link_imp_link_mod; eauto.
+  Qed.
+
+  Definition imp_initial_state (src : Imp.programL) :=
+    (ModL.compile (ImpMod.get_modL src)).(initial_state).
+
+  Lemma single_compile_behavior_improves
+        (src: Imp.programL) (tgt: Csharpminor.program) srcst tgtst
+        (COMP: compile src = OK tgt)
+        (SINIT: srcst = imp_initial_state src)
+        (TINIT: Csharpminor.initial_state tgt tgtst)
+    :
+      <<IMPROVES: @improves2 _ (Csharpminor.semantics tgt) srcst tgtst>>.
+  Proof.
+  Admitted.
+
+  Definition src_initial_state (src : ModL.t) :=
+    (ModL.compile src).(initial_state).
+
+  Theorem compile_behavior_improves
+          (src_list : list Imp.program) srcl tgt_list tgtl srcst tgtst
+          (COMP: let src_list_lift := List.map Imp.lift src_list in
+                 compile_list src_list_lift tgt_list)
+          (LINKSRC: let src_list_mod := List.map ImpMod.get_mod src_list in
+                    Mod.add_list (Mem :: src_list_mod) = srcl)
+          (LINKTGT: link_csm_list tgt_list = Some tgtl)
+          (SINIT: srcst = src_initial_state srcl)
+          (TINIT: Csharpminor.initial_state tgtl tgtst)
+    :
+      <<IMPROVES: @improves2 _ (Csharpminor.semantics tgtl) srcst tgtst>>.
+  Proof.
+  Admitted.
+
+End PROOFALL.
